src/PredCalc/CommonModels.v
@@ -5,14 +5,12 @@ From MRC Require Import Tactics.
 From MRC Require Import Stdppp.
 From MRC Require Import Model.
 From MRC Require Import PredCalc.Basic.
+Import EqNotations.
 
-Class ModelWithSum (M : model) := {
-  sum_fdef : @fdef (value M) (value_ty M) (hastype M);
-  sum_fdef_fdefs : fdefs M !! "+"%string = Some sum_fdef;
-}.
+Class ModelWithSum (M : model) := sum_sym : model_fsym M.
 
-Definition term_sum {M} `{ModelWithSum M} (t u : term (value M)) : term (value M) :=
-  TApp "+" [t; u].
+Definition term_sum {M} `{ModelWithSum M} (t u : termM M) : termM M :=
+  TApp sum_sym [t; u].
 
 Notation "t + u" := (term_sum t u)
                       (in custom term at level 50,
@@ -20,55 +18,47 @@ Notation "t + u" := (term_sum t u)
                           u custom term,
                           left associativity) : refiney_scope.
 
-Class ModelWithSub (M : model) := {
-  sub_fdef : @fdef (value M) (value_ty M) (hastype M);
-  sub_fdef_fdefs : fdefs M !! "*"%string = Some sub_fdef;
-}.
+Class ModelWithSub (M : model) := sub_sym : model_fsym M.
 
-Definition term_sub {M} `{ModelWithSum M} (t u : term (value M)) : term (value M) :=
-  TApp "-" [t; u].
+Definition term_sub {M} `{ModelWithSub M} (t u : termM M) : termM M :=
+  TApp sub_sym [t; u].
 
-Notation "t - u" := (TApp "-" (@cons term t (@cons term u nil)))
+Notation "t - u" := (term_sub t u)
                       (in custom term at level 50,
                           t custom term,
                           u custom term,
                           left associativity) : refiney_scope.
 
-Class ModelWithMul (M : model) := {
-  mul_fdef : @fdef (value M) (value_ty M) (hastype M);
-  mul_fdef_fdefs : fdefs M !! "*"%string = Some mul_fdef;
-}.
+Class ModelWithMul (M : model) := mul_sym : model_fsym M.
+Definition term_mul {M} `{ModelWithMul M} (t u : termM M) : termM M :=
+  TApp mul_sym [t; u].
 
-Definition term_mul {M} `{ModelWithSum M} (t u : term (value M)) : term (value M) :=
-  TApp "*" [t; u].
-
-Notation "t * u" := (TApp "*" (@cons term t (@cons term u nil)))
+Notation "t * u" := (term_mul t u)
                       (in custom term at level 50,
                           t custom term,
                           u custom term,
                           left associativity) : refiney_scope.
 
 Class ModelWithOrder (M : model) := {
-  lt_pdef : @pdef (value M);
-  lt_pdef_arity : pdef_arity lt_pdef = 2;
-  lt_pdef_pdefs : pdefs M !! "<"%string = Some lt_pdef;
+  lt_sym : model_psym M;
+  lt_pdef_arity : pdef_arity (pdefs M lt_sym) = 2;
 }.
 
 Definition lt_pdef_rel {M : model} (v1 v2 : value M) `{ModelWithOrder M} : Prop.
 Proof.
-  pose proof (pdef_rel lt_pdef). rewrite lt_pdef_arity in X. apply (X [# v1; v2]).
+  pose proof (pdef_rel (pdefs M lt_sym)). rewrite lt_pdef_arity in X. apply (X [# v1; v2]).
 Defined.
 
-Definition term_lt {M} `{ModelWithOrder M} (t u : term (value M)) : formulaM M :=
-  FAtom (AT_Pred ("<") [t; u]).
+Definition term_lt {M} `{ModelWithOrder M} (t u : termM M) : formulaM M :=
+  FAtom (AT_Pred lt_sym [t; u]).
 
-Definition term_le {M} `{ModelWithOrder M} (t u : term (value M)) : formulaM M :=
-  FAnd (FAtom (AT_Pred ("≤") [t; u])) (FAtom (AT_Eq t u)).
+Definition term_le {M} `{ModelWithOrder M} (t u : termM M) : formulaM M :=
+  FOr (term_lt t u) (FAtom (AT_Eq t u)).
 
-Definition term_gt {M} `{ModelWithOrder M} (t u : term (value M)) : formulaM M :=
+Definition term_gt {M} `{ModelWithOrder M} (t u : termM M) : formulaM M :=
   term_lt u t.
 
-Definition term_ge {M} `{ModelWithOrder M} (t u : term (value M)) : formulaM M :=
+Definition term_ge {M} `{ModelWithOrder M} (t u : termM M) : formulaM M :=
   term_le u t.
 
 Notation "t = u" := (FAtom (AT_Eq t u))
@@ -117,17 +107,17 @@ Class ModelWithNat (M : model) := {
   nat_sum_fdef : ∀ v1 v2 n1 n2,
       value_to_nat v1 = Some n1 →
       value_to_nat v2 = Some n2 →
-      fdef_rel sum_fdef [v1; v2] (nat_to_value (n1 + n2));
+      fn_eval sum_sym [v1; v2] (nat_to_value (n1 + n2));
   nat_with_sub :: ModelWithSub M;
   nat_sub_fdef : ∀ v1 v2 n1 n2,
       value_to_nat v1 = Some n1 →
       value_to_nat v2 = Some n2 →
-      fdef_rel sub_fdef [v1; v2] (nat_to_value (n1 - n2));
+      fn_eval sub_sym [v1; v2] (nat_to_value (n1 - n2));
   nat_with_mul :: ModelWithMul M;
   nat_mul_fdef : ∀ v1 v2 n1 n2,
       value_to_nat v1 = Some n1 →
       value_to_nat v2 = Some n2 →
-      fdef_rel mul_fdef [v1; v2] (nat_to_value (n1 * n2));
+      fn_eval mul_sym [v1; v2] (nat_to_value (n1 * n2));
   nat_with_order :: ModelWithOrder M;
   nat_lt_pdef : ∀ v1 v2 n1 n2,
       value_to_nat v1 = Some n1 →
