src/PredCalc/SetSolver.v
@@ -17,6 +17,7 @@ Section set_solver.
   Context {M : model}.
   Local Notation value := (value M).
   Local Notation value_ty := (value_ty M).
+  Local Notation sym := (model_symbols M).
   Local Notation term := (termM M).
   Local Notation formula := (formulaM M).
 
@@ -25,7 +26,7 @@ Section set_solver.
   Implicit Types ts : list term.
 
   Global Instance set_unfold_elem_of_term_fvars x ts P1 P2 :
-    (∀ t, SetUnfoldElemOf x (@term_fvars value t) (P1 t)) →
+    (∀ t, SetUnfoldElemOf x (@term_fvars value sym t) (P1 t)) →
     (∀ t, SetUnfoldElemOf t ts (P2 t)) →
     SetUnfoldElemOf x
       (⋃ (term_fvars <$> ts))
@@ -37,7 +38,7 @@ Section set_solver.
   Global Instance set_unfold_elem_of_term_fvars_of_initial_vars x w Q :
     SetUnfoldElemOf (to_final_var x) w Q →
     SetUnfoldElemOf x
-      (⋃ (term_fvars <$> (@TVar value <$> (initial_var_of <$> w))))
+      (⋃ (term_fvars <$> (@TVar value sym <$> (initial_var_of <$> w))))
       (¬ var_final x ∧ Q).
   Proof with auto.
     constructor. set_unfold. split.
@@ -51,7 +52,7 @@ Section set_solver.
   Global Instance set_unfold_elem_of_term_fvars_of_vars x w Q :
     SetUnfoldElemOf (to_final_var x) w Q →
     SetUnfoldElemOf x
-      (⋃ (term_fvars <$> (@TVar value <$> (as_var <$> w))))
+      (⋃ (term_fvars <$> (@TVar value sym <$> (as_var <$> w))))
       (var_final x ∧ Q).
   Proof with auto.
     constructor. set_unfold. split.
@@ -180,7 +181,7 @@ Section set_solver.
   Global Instance set_unfold_elem_of_fvars_FEqList x ts1 ts2 Hsl Q1 Q2 :
     SetUnfoldElemOf x (⋃ (term_fvars <$> ts1)) Q1 →
     SetUnfoldElemOf x (⋃ (term_fvars <$> ts2)) Q2 →
-    SetUnfoldElemOf x (formula_fvars (@FEqList _ value_ty ts1 ts2 Hsl)) (Q1 ∨ Q2).
+    SetUnfoldElemOf x (formula_fvars (@FEqList _ value_ty _ ts1 ts2 Hsl)) (Q1 ∨ Q2).
   Proof with auto. intros. constructor. rewrite fvars_eqlist. set_solver. Qed.
 
 End set_solver.
